@prefix : <https://bbp.epfl.ch/ontologies/core/efeatures/> .
@prefix owl: <http://www.w3.org/2002/07/owl#> .
@prefix rdf: <http://www.w3.org/1999/02/22-rdf-syntax-ns#> .
@prefix xml: <http://www.w3.org/XML/1998/namespace> .
@prefix xsd: <http://www.w3.org/2001/XMLSchema#> .
@prefix rdfs: <http://www.w3.org/2000/01/rdf-schema#> .
@base <https://bbp.epfl.ch/ontologies/core/efeatures> .

<https://bbp.epfl.ch/ontologies/core/efeatures> rdf:type owl:Ontology ;
                                                 rdfs:label "Electrophysiological Features Ontology"@en .

#################################################################
#    Annotation properties
#################################################################

###  http://www.w3.org/2004/02/skos/core#altLabel
<http://www.w3.org/2004/02/skos/core#altLabel> rdf:type owl:AnnotationProperty .


###  http://www.w3.org/2004/02/skos/core#definition
<http://www.w3.org/2004/02/skos/core#definition> rdf:type owl:AnnotationProperty .


###  https://bbp.epfl.ch/ontologies/core/efeatures/efel_id
:efel_id rdf:type owl:AnnotationProperty ;
         rdfs:label "efel_id"@en .


###  https://bbp.epfl.ch/ontologies/core/efeatures/efel_namespace
:efel_namespace rdf:type owl:AnnotationProperty ;
                rdfs:label "efel_namespace"@en .


###  https://neuroshapes.org/units
<https://neuroshapes.org/units> rdf:type owl:AnnotationProperty ;
                                rdfs:label "units"@en .


#################################################################
#    Classes
#################################################################

###  https://bbp.epfl.ch/ontologies/core/bmo/NeuronElectrophysiologicalFeature
<https://bbp.epfl.ch/ontologies/core/bmo/NeuronElectrophysiologicalFeature> rdf:type owl:Class ;
                                                                            rdfs:label "Neuron Electrophysiological Feature"@en .


###  https://bbp.epfl.ch/ontologies/core/efeatures/ADPAmplitude
:ADPAmplitude rdf:type owl:Class ;
              rdfs:subClassOf <https://bbp.epfl.ch/ontologies/core/bmo/NeuronElectrophysiologicalFeature> ,
                              :NeuroElectroNeuronElectrophysiologicalFeature ;
              rdfs:label "ADP Amplitude"@en ;
              <http://www.w3.org/2004/02/skos/core#definition> "Amplitude from first AP onset to maximum voltage, typically more depolarized than the resting membrane potential"@en ;
              <https://neuroshapes.org/units> "mV" .


###  https://bbp.epfl.ch/ontologies/core/efeatures/ADPDuration
:ADPDuration rdf:type owl:Class ;
             rdfs:subClassOf <https://bbp.epfl.ch/ontologies/core/bmo/NeuronElectrophysiologicalFeature> ,
                             :NeuroElectroNeuronElectrophysiologicalFeature ;
             rdfs:label "ADP Duration"@en ;
             <http://www.w3.org/2004/02/skos/core#definition> "Duration from first AP onset to maximum ADP"@en ;
             <https://neuroshapes.org/units> "ms" .


###  https://bbp.epfl.ch/ontologies/core/efeatures/AHPAmplitude
:AHPAmplitude rdf:type owl:Class ;
              rdfs:subClassOf <https://bbp.epfl.ch/ontologies/core/bmo/NeuronElectrophysiologicalFeature> ,
                              :NeuroElectroNeuronElectrophysiologicalFeature ;
              rdfs:label "AHP Amplitude"@en ;
              <http://www.w3.org/2004/02/skos/core#definition> "Calculated as the voltage difference between AP threshold and AP trough. Commonly defined using first AP in train at rheobase current."@en ;
              <https://neuroshapes.org/units> "mV" .


###  https://bbp.epfl.ch/ontologies/core/efeatures/AHPAmplitudeFromResting
:AHPAmplitudeFromResting rdf:type owl:Class ;
                         rdfs:subClassOf <https://bbp.epfl.ch/ontologies/core/bmo/NeuronElectrophysiologicalFeature> ,
                                         :NeuroElectroNeuronElectrophysiologicalFeature ;
                         rdfs:label "AHP Amplitude From Resting"@en ;
                         <http://www.w3.org/2004/02/skos/core#definition> "Calculated as the voltage difference between resting or baseline voltages and AP trough. Commonly defined using first AP in train at rheobase current."@en ;
                         <https://neuroshapes.org/units> "mV" .


###  https://bbp.epfl.ch/ontologies/core/efeatures/AHPDuration
:AHPDuration rdf:type owl:Class ;
             rdfs:subClassOf <https://bbp.epfl.ch/ontologies/core/bmo/NeuronElectrophysiologicalFeature> ,
                             :NeuroElectroNeuronElectrophysiologicalFeature ;
             rdfs:label "AHP Duration"@en ;
             <http://www.w3.org/2004/02/skos/core#definition> "Duration of AP after-hyperpolarization, not explicitly referred to by author as either fast or slow"@en ;
             <https://neuroshapes.org/units> "ms" .


###  https://bbp.epfl.ch/ontologies/core/efeatures/AHPVoltage
:AHPVoltage rdf:type owl:Class ;
            rdfs:subClassOf <https://bbp.epfl.ch/ontologies/core/bmo/NeuronElectrophysiologicalFeature> ,
                            :NeuroElectroNeuronElectrophysiologicalFeature ;
            rdfs:label "AHP Voltage"@en ;
            <http://www.w3.org/2004/02/skos/core#definition> "Calculated as minimum voltage value during an AHP. Commonly defined using first AP in train at rheobase current."@en ;
            <https://neuroshapes.org/units> "mV" .


###  https://bbp.epfl.ch/ontologies/core/efeatures/AccessResistance
:AccessResistance rdf:type owl:Class ;
                  rdfs:subClassOf <https://bbp.epfl.ch/ontologies/core/bmo/NeuronElectrophysiologicalFeature> ,
                                  :NeuroElectroNeuronElectrophysiologicalFeature ;
                  rdfs:label "Access Resistance"@en ;
                  <http://www.w3.org/2004/02/skos/core#definition> "Sum of the electrode resistance and the resistance at the electrode-cell junction"@en ;
                  <https://neuroshapes.org/units> "M\\ohm" .


###  https://bbp.epfl.ch/ontologies/core/efeatures/AdaptationPercent1
:AdaptationPercent1 rdf:type owl:Class ;
                    rdfs:subClassOf <https://bbp.epfl.ch/ontologies/core/bmo/NeuronElectrophysiologicalFeature> ,
                                    :NeuroElectroNeuronElectrophysiologicalFeature ;
                    rdfs:label "Adaptation Percent1"@en ;
                    <http://www.w3.org/2004/02/skos/core#altLabel> "adaptation percent (first/last ISI)"@en ;
                    <http://www.w3.org/2004/02/skos/core#definition> "Percentage of durations between early and late AP inter-spike intervals in an AP train"@en ;
                    <https://neuroshapes.org/units> "Unitless" .


###  https://bbp.epfl.ch/ontologies/core/efeatures/AdaptationPercent2
:AdaptationPercent2 rdf:type owl:Class ;
                    rdfs:subClassOf <https://bbp.epfl.ch/ontologies/core/bmo/NeuronElectrophysiologicalFeature> ,
                                    :NeuroElectroNeuronElectrophysiologicalFeature ;
                    rdfs:label "Adaptation Percent2"@en ;
                    <http://www.w3.org/2004/02/skos/core#altLabel> "adaptation percent (last/first ISI)"@en ;
                    <http://www.w3.org/2004/02/skos/core#definition> "Percentage of durations between late and early AP inter-spike intervals in an AP train"@en ;
                    <https://neuroshapes.org/units> "Unitless" .


###  https://bbp.epfl.ch/ontologies/core/efeatures/AdaptationPercent3
:AdaptationPercent3 rdf:type owl:Class ;
                    rdfs:subClassOf <https://bbp.epfl.ch/ontologies/core/bmo/NeuronElectrophysiologicalFeature> ,
                                    :NeuroElectroNeuronElectrophysiologicalFeature ;
                    rdfs:label "Adaptation Percent3"@en ;
                    <http://www.w3.org/2004/02/skos/core#altLabel> "adaptation percent (1 – first/last ISI)"@en ;
                    <http://www.w3.org/2004/02/skos/core#definition> "1 minus ratio of durations between early and late AP inter-spike intervals in an AP train, normalized to a percent"@en ;
                    <https://neuroshapes.org/units> "Unitless" .


###  https://bbp.epfl.ch/ontologies/core/efeatures/AdaptationRatio
:AdaptationRatio rdf:type owl:Class ;
                 rdfs:subClassOf <https://bbp.epfl.ch/ontologies/core/bmo/NeuronElectrophysiologicalFeature> ,
                                 :NeuroElectroNeuronElectrophysiologicalFeature ;
                 rdfs:label "Adaptation Ratio"@en ;
                 <http://www.w3.org/2004/02/skos/core#definition> "Ratio of durations between early and late AP inter-spike intervals in an AP train"@en ;
                 <https://neuroshapes.org/units> "Unitless" .


###  https://bbp.epfl.ch/ontologies/core/efeatures/AdaptationRatio1
:AdaptationRatio1 rdf:type owl:Class ;
                  rdfs:subClassOf <https://bbp.epfl.ch/ontologies/core/bmo/NeuronElectrophysiologicalFeature> ,
                                  :NeuroElectroNeuronElectrophysiologicalFeature ;
                  rdfs:label "Adaptation Ratio1"@en ;
                  <http://www.w3.org/2004/02/skos/core#altLabel> "adaptation ratio (last/first ISI)"@en ;
                  <http://www.w3.org/2004/02/skos/core#definition> "Ratio of durations between late and early AP inter-spike intervals in an AP train"@en ;
                  <https://neuroshapes.org/units> "Unitless" .


###  https://bbp.epfl.ch/ontologies/core/efeatures/AdaptationRatio2
:AdaptationRatio2 rdf:type owl:Class ;
                  rdfs:subClassOf <https://bbp.epfl.ch/ontologies/core/bmo/NeuronElectrophysiologicalFeature> ,
                                  :NeuroElectroNeuronElectrophysiologicalFeature ;
                  rdfs:label "Adaptation Ratio2"@en ;
                  <http://www.w3.org/2004/02/skos/core#altLabel> "adaptation ratio (1 – first/last ISI)"@en ;
                  <http://www.w3.org/2004/02/skos/core#definition> "1 minus ratio of durations between early and late AP inter-spike intervals in an AP train"@en ;
                  <https://neuroshapes.org/units> "Unitless" .


###  https://bbp.epfl.ch/ontologies/core/efeatures/AdaptationRatio3
:AdaptationRatio3 rdf:type owl:Class ;
                  rdfs:subClassOf <https://bbp.epfl.ch/ontologies/core/bmo/NeuronElectrophysiologicalFeature> ,
                                  :NeuroElectroNeuronElectrophysiologicalFeature ;
                  rdfs:label "Adaptation Ratio3"@en ;
                  <http://www.w3.org/2004/02/skos/core#altLabel> "adaptation ratio (other)"@en ;
                  <http://www.w3.org/2004/02/skos/core#definition> "Adaptation ratio, percent, index but not otherwise characterizable to an existing sub-definition"@en ;
                  <https://neuroshapes.org/units> "Unitless" .


###  https://bbp.epfl.ch/ontologies/core/efeatures/CellCapacitance
:CellCapacitance rdf:type owl:Class ;
                 rdfs:subClassOf <https://bbp.epfl.ch/ontologies/core/bmo/NeuronElectrophysiologicalFeature> ,
                                 :NeuroElectroNeuronElectrophysiologicalFeature ;
                 rdfs:label "Cell Capacitance"@en ;
                 <http://www.w3.org/2004/02/skos/core#definition> "Neuron capacitance, typically measured by dividing membrane time constant by membrane resistance"@en ;
                 <https://neuroshapes.org/units> "pF" .


###  https://bbp.epfl.ch/ontologies/core/efeatures/CellDiameter
:CellDiameter rdf:type owl:Class ;
              rdfs:subClassOf <https://bbp.epfl.ch/ontologies/core/bmo/NeuronElectrophysiologicalFeature> ,
                              :NeuroElectroNeuronElectrophysiologicalFeature ;
              rdfs:label "Cell Diameter"@en ;
              <http://www.w3.org/2004/02/skos/core#definition> "Diameter of the cell soma"@en ;
              <https://neuroshapes.org/units> "um" .


###  https://bbp.epfl.ch/ontologies/core/efeatures/CellSurfaceArea
:CellSurfaceArea rdf:type owl:Class ;
                 rdfs:subClassOf <https://bbp.epfl.ch/ontologies/core/bmo/NeuronElectrophysiologicalFeature> ,
                                 :NeuroElectroNeuronElectrophysiologicalFeature ;
                 rdfs:label "Cell Surface Area"@en ;
                 <http://www.w3.org/2004/02/skos/core#definition> "Cross-sectional area of the cell"@en ;
                 <https://neuroshapes.org/units> "m" .


###  https://bbp.epfl.ch/ontologies/core/efeatures/FISlope
:FISlope rdf:type owl:Class ;
         rdfs:subClassOf <https://bbp.epfl.ch/ontologies/core/bmo/NeuronElectrophysiologicalFeature> ,
                         :NeuroElectroNeuronElectrophysiologicalFeature ;
         rdfs:label "FI Slope"@en ;
         <http://www.w3.org/2004/02/skos/core#definition> "Slope of the frequency-current relationship"@en ;
         <https://neuroshapes.org/units> "Hz/nA" .


###  https://bbp.epfl.ch/ontologies/core/efeatures/FastAHPAmplitude
:FastAHPAmplitude rdf:type owl:Class ;
                  rdfs:subClassOf <https://bbp.epfl.ch/ontologies/core/bmo/NeuronElectrophysiologicalFeature> ,
                                  :NeuroElectroNeuronElectrophysiologicalFeature ;
                  rdfs:label "Fast AHP Amplitude"@en ;
                  <http://www.w3.org/2004/02/skos/core#definition> "Calculated as the difference between AP threshold and AP trough, explictly refered to by author as fast."@en ;
                  <https://neuroshapes.org/units> "mV" .


###  https://bbp.epfl.ch/ontologies/core/efeatures/FastAHPAmplitudeFromResting
:FastAHPAmplitudeFromResting rdf:type owl:Class ;
                             rdfs:subClassOf <https://bbp.epfl.ch/ontologies/core/bmo/NeuronElectrophysiologicalFeature> ,
                                             :NeuroElectroNeuronElectrophysiologicalFeature ;
                             rdfs:label "Fast AHP Amplitude From Resting"@en ;
                             <http://www.w3.org/2004/02/skos/core#definition> "Calculated as the difference between resting or baseline voltages and AP trough, explictly refered to by author as fast."@en ;
                             <https://neuroshapes.org/units> "mV" .


###  https://bbp.epfl.ch/ontologies/core/efeatures/FastAHPDuration
:FastAHPDuration rdf:type owl:Class ;
                 rdfs:subClassOf <https://bbp.epfl.ch/ontologies/core/bmo/NeuronElectrophysiologicalFeature> ,
                                 :NeuroElectroNeuronElectrophysiologicalFeature ;
                 rdfs:label "Fast AHP Duration"@en ;
                 <http://www.w3.org/2004/02/skos/core#definition> "Duration of AP after-hyperpolarization, explictly refered to by author as fast"@en ;
                 <https://neuroshapes.org/units> "ms" .


###  https://bbp.epfl.ch/ontologies/core/efeatures/FastAHPVoltage
:FastAHPVoltage rdf:type owl:Class ;
                rdfs:subClassOf <https://bbp.epfl.ch/ontologies/core/bmo/NeuronElectrophysiologicalFeature> ,
                                :NeuroElectroNeuronElectrophysiologicalFeature ;
                rdfs:label "Fast AHP Voltage"@en ;
                <http://www.w3.org/2004/02/skos/core#definition> "Calculated as the AHP absolute voltage, explictly refered to by author as fast."@en ;
                <https://neuroshapes.org/units> "mV" .


###  https://bbp.epfl.ch/ontologies/core/efeatures/FiringFrequency
:FiringFrequency rdf:type owl:Class ;
                 rdfs:subClassOf <https://bbp.epfl.ch/ontologies/core/bmo/NeuronElectrophysiologicalFeature> ,
                                 :NeuroElectroNeuronElectrophysiologicalFeature ;
                 rdfs:label "Firing Frequency"@en ;
                 <http://www.w3.org/2004/02/skos/core#definition> "AP discharge rate, AP frequency, spike rate, firing rate, spike frequency, mean firing rate, steady state firing rate, average firing rate, steady firing rate"@en ;
                 <https://neuroshapes.org/units> "Hz" .


###  https://bbp.epfl.ch/ontologies/core/efeatures/FirstSpikeLatency
:FirstSpikeLatency rdf:type owl:Class ;
                   rdfs:subClassOf <https://bbp.epfl.ch/ontologies/core/bmo/NeuronElectrophysiologicalFeature> ,
                                   :NeuroElectroNeuronElectrophysiologicalFeature ;
                   rdfs:label "First Spike Latency"@en ;
                   <http://www.w3.org/2004/02/skos/core#definition> "Duration to first AP following a depolarizing current step of fixed amplitude"@en ;
                   <https://neuroshapes.org/units> "ms" .


###  https://bbp.epfl.ch/ontologies/core/efeatures/InputResistance
:InputResistance rdf:type owl:Class ;
                 rdfs:subClassOf <https://bbp.epfl.ch/ontologies/core/bmo/NeuronElectrophysiologicalFeature> ,
                                 :NeuroElectroNeuronElectrophysiologicalFeature ;
                 rdfs:label "Input Resistance"@en ;
                 <http://www.w3.org/2004/02/skos/core#definition> "Input resistance measured at steady-state voltage response to current injection"@en ;
                 <https://neuroshapes.org/units> "M\\ohm" .


###  https://bbp.epfl.ch/ontologies/core/efeatures/MaximumFiringRate
:MaximumFiringRate rdf:type owl:Class ;
                   rdfs:subClassOf <https://bbp.epfl.ch/ontologies/core/bmo/NeuronElectrophysiologicalFeature> ,
                                   :NeuroElectroNeuronElectrophysiologicalFeature ;
                   rdfs:label "Maximum Firing Rate"@en ;
                   <http://www.w3.org/2004/02/skos/core#definition> "Maximum observed AP discharge rate"@en ;
                   <https://neuroshapes.org/units> "Hz" .


###  https://bbp.epfl.ch/ontologies/core/efeatures/MediumAHPAmplitude
:MediumAHPAmplitude rdf:type owl:Class ;
                    rdfs:subClassOf <https://bbp.epfl.ch/ontologies/core/bmo/NeuronElectrophysiologicalFeature> ,
                                    :NeuroElectroNeuronElectrophysiologicalFeature ;
                    rdfs:label "Medium AHP Amplitude"@en ;
                    <http://www.w3.org/2004/02/skos/core#definition> "Calculated as the difference between AP threshold and AP trough, explictly refered to by author as medium"@en ;
                    <https://neuroshapes.org/units> "mV" .


###  https://bbp.epfl.ch/ontologies/core/efeatures/MediumAHPAmplitudeFromResting
:MediumAHPAmplitudeFromResting rdf:type owl:Class ;
                               rdfs:subClassOf <https://bbp.epfl.ch/ontologies/core/bmo/NeuronElectrophysiologicalFeature> ,
                                               :NeuroElectroNeuronElectrophysiologicalFeature ;
                               rdfs:label "Medium AHP Amplitude From Resting"@en ;
                               <http://www.w3.org/2004/02/skos/core#definition> "Calculated as the difference between resting or baseline voltages and AP trough, explictly refered to by author as medium"@en ;
                               <https://neuroshapes.org/units> "mV" .


###  https://bbp.epfl.ch/ontologies/core/efeatures/MediumAHPDuration
:MediumAHPDuration rdf:type owl:Class ;
                   rdfs:subClassOf <https://bbp.epfl.ch/ontologies/core/bmo/NeuronElectrophysiologicalFeature> ,
                                   :NeuroElectroNeuronElectrophysiologicalFeature ;
                   rdfs:label "Medium AHP Duration"@en ;
                   <http://www.w3.org/2004/02/skos/core#definition> "Duration of AP after-hyperpolarization, explictly refered to by author as medium"@en ;
                   <https://neuroshapes.org/units> "ms" .


###  https://bbp.epfl.ch/ontologies/core/efeatures/MediumAHPVoltage
:MediumAHPVoltage rdf:type owl:Class ;
                  rdfs:subClassOf <https://bbp.epfl.ch/ontologies/core/bmo/NeuronElectrophysiologicalFeature> ,
                                  :NeuroElectroNeuronElectrophysiologicalFeature ;
                  rdfs:label "Medium AHP Voltage"@en ;
                  <http://www.w3.org/2004/02/skos/core#definition> "Calculated as the AHP absolute voltage, explictly refered to by author as medium."@en ;
                  <https://neuroshapes.org/units> "mV" .


###  https://bbp.epfl.ch/ontologies/core/efeatures/MembraneTimeConstant
:MembraneTimeConstant rdf:type owl:Class ;
                      rdfs:subClassOf <https://bbp.epfl.ch/ontologies/core/bmo/NeuronElectrophysiologicalFeature> ,
                                      :NeuroElectroNeuronElectrophysiologicalFeature ;
                      rdfs:label "Membrane Time Constant"@en ;
                      <http://www.w3.org/2004/02/skos/core#definition> "Time constant for the membrane to repolarize after a small current injection of fixed amplitude and duration"@en ;
                      <https://neuroshapes.org/units> "ms" .


###  https://bbp.epfl.ch/ontologies/core/efeatures/NeuroElectroNeuronElectrophysiologicalFeature
:NeuroElectroNeuronElectrophysiologicalFeature rdf:type owl:Class ;
                                               rdfs:label "NeuroElectro Neuron Electrophysiological Feature"@en .


###  https://bbp.epfl.ch/ontologies/core/efeatures/Other
:Other rdf:type owl:Class ;
       rdfs:subClassOf <https://bbp.epfl.ch/ontologies/core/bmo/NeuronElectrophysiologicalFeature> ,
                       :NeuroElectroNeuronElectrophysiologicalFeature ;
       rdfs:label "Other"@en ;
       <http://www.w3.org/2004/02/skos/core#definition> "A catch-all property to reflect any properties which are not already explicitly defined"@en ;
       <https://neuroshapes.org/units> "Unitless" .


###  https://bbp.epfl.ch/ontologies/core/efeatures/RestingMembranePotential
:RestingMembranePotential rdf:type owl:Class ;
                          rdfs:subClassOf <https://bbp.epfl.ch/ontologies/core/bmo/NeuronElectrophysiologicalFeature> ,
                                          :NeuroElectroNeuronElectrophysiologicalFeature ;
                          rdfs:label "Resting Membrane Potential"@en ;
                          <http://www.w3.org/2004/02/skos/core#definition> "Membrane potential at the onset of whole-cell recording"@en ;
                          <https://neuroshapes.org/units> "mV" .


###  https://bbp.epfl.ch/ontologies/core/efeatures/Rheobase
:Rheobase rdf:type owl:Class ;
          rdfs:subClassOf <https://bbp.epfl.ch/ontologies/core/bmo/NeuronElectrophysiologicalFeature> ,
                          :NeuroElectroNeuronElectrophysiologicalFeature ;
          rdfs:label "Rheobase"@en ;
          <http://www.w3.org/2004/02/skos/core#definition> "Minimum current injected somatically required to fire AP"@en ;
          <https://neuroshapes.org/units> "pA" .


###  https://bbp.epfl.ch/ontologies/core/efeatures/SagAmplitude2
:SagAmplitude2 rdf:type owl:Class ;
               rdfs:subClassOf <https://bbp.epfl.ch/ontologies/core/bmo/NeuronElectrophysiologicalFeature> ,
                               :NeuroElectroNeuronElectrophysiologicalFeature ;
               rdfs:label "Sag Amplitude2"@en ;
               <http://www.w3.org/2004/02/skos/core#definition> "Absolute difference between the steady state decrease in the voltage and the largest decrease in voltage following a hyperpolarizing current step."^^xsd:string ;
               <https://neuroshapes.org/units> "mV"^^xsd:string .


###  https://bbp.epfl.ch/ontologies/core/efeatures/SagRatio
:SagRatio rdf:type owl:Class ;
          rdfs:subClassOf <https://bbp.epfl.ch/ontologies/core/bmo/NeuronElectrophysiologicalFeature> ,
                          :NeuroElectroNeuronElectrophysiologicalFeature ;
          rdfs:label "Sag Ratio"@en ;
          <http://www.w3.org/2004/02/skos/core#definition> "Ratio between the steady state decrease in the voltage and the largest decrease in voltage following a hyperpolarizing current step."@en ;
          <https://neuroshapes.org/units> "Unitless" .


###  https://bbp.epfl.ch/ontologies/core/efeatures/SlowAHPAmplitude
:SlowAHPAmplitude rdf:type owl:Class ;
                  rdfs:subClassOf <https://bbp.epfl.ch/ontologies/core/bmo/NeuronElectrophysiologicalFeature> ,
                                  :NeuroElectroNeuronElectrophysiologicalFeature ;
                  rdfs:label "Slow AHP Amplitude"@en ;
                  <http://www.w3.org/2004/02/skos/core#definition> "Calculated as the difference between AP threshold and AP trough, explictly refered to by author as slow"@en ;
                  <https://neuroshapes.org/units> "mV" .


###  https://bbp.epfl.ch/ontologies/core/efeatures/SlowAHPAmplitudeFromResting
:SlowAHPAmplitudeFromResting rdf:type owl:Class ;
                             rdfs:subClassOf <https://bbp.epfl.ch/ontologies/core/bmo/NeuronElectrophysiologicalFeature> ,
                                             :NeuroElectroNeuronElectrophysiologicalFeature ;
                             rdfs:label "Slow AHP Amplitude From Resting"@en ;
                             <http://www.w3.org/2004/02/skos/core#definition> "Calculated as the difference between resting or baseline voltages and AP trough, explictly refered to by author as slow"@en ;
                             <https://neuroshapes.org/units> "mV" .


###  https://bbp.epfl.ch/ontologies/core/efeatures/SlowAHPDuration
:SlowAHPDuration rdf:type owl:Class ;
                 rdfs:subClassOf <https://bbp.epfl.ch/ontologies/core/bmo/NeuronElectrophysiologicalFeature> ,
                                 :NeuroElectroNeuronElectrophysiologicalFeature ;
                 rdfs:label "Slow AHP Duration"@en ;
                 <http://www.w3.org/2004/02/skos/core#definition> "Duration of AP after-hyperpolarization, explictly refered to by author as slow"@en ;
                 <https://neuroshapes.org/units> "ms" .


###  https://bbp.epfl.ch/ontologies/core/efeatures/SlowAHPVoltage
:SlowAHPVoltage rdf:type owl:Class ;
                rdfs:subClassOf <https://bbp.epfl.ch/ontologies/core/bmo/NeuronElectrophysiologicalFeature> ,
                                :NeuroElectroNeuronElectrophysiologicalFeature ;
                rdfs:label "Slow AHP Voltage"@en ;
                <http://www.w3.org/2004/02/skos/core#definition> "Calculated as the AHP absolute voltage, explictly refered to by author as slow."@en ;
                <https://neuroshapes.org/units> "mV" .


###  https://bbp.epfl.ch/ontologies/core/efeatures/SpikeAmplitude
:SpikeAmplitude rdf:type owl:Class ;
                rdfs:subClassOf <https://bbp.epfl.ch/ontologies/core/bmo/NeuronElectrophysiologicalFeature> ,
                                :NeuroElectroNeuronElectrophysiologicalFeature ;
                rdfs:label "Spike Amplitude"@en ;
                <http://www.w3.org/2004/02/skos/core#definition> "Voltage indicating height of action potential. Usually calculated as the difference between AP peak and AP threshold voltages. Commonly measured using first AP in train at rheobase current."@en ;
                <https://neuroshapes.org/units> "mV" .


###  https://bbp.epfl.ch/ontologies/core/efeatures/SpikeAmplitudeFromResting
:SpikeAmplitudeFromResting rdf:type owl:Class ;
                           rdfs:subClassOf <https://bbp.epfl.ch/ontologies/core/bmo/NeuronElectrophysiologicalFeature> ,
                                           :NeuroElectroNeuronElectrophysiologicalFeature ;
                           rdfs:label "Spike Amplitude From Resting"@en ;
                           <http://www.w3.org/2004/02/skos/core#definition> "Voltage indicating height of action potential, calculated as the difference between AP peak and resting or baseline voltages. Commonly measured using first AP in train at rheobase current."@en ;
                           <https://neuroshapes.org/units> "mV" .


###  https://bbp.epfl.ch/ontologies/core/efeatures/SpikeAmplitudeFromTrough
:SpikeAmplitudeFromTrough rdf:type owl:Class ;
                          rdfs:subClassOf <https://bbp.epfl.ch/ontologies/core/bmo/NeuronElectrophysiologicalFeature> ,
                                          :NeuroElectroNeuronElectrophysiologicalFeature ;
                          rdfs:label "Spike Amplitude From Trough"@en ;
                          <http://www.w3.org/2004/02/skos/core#definition> "Voltage indicating height of action potential, calculated as the difference between AP peak and AHP trough voltages. Commonly measured using first AP in train at rheobase current."@en ;
                          <https://neuroshapes.org/units> "mV" .


###  https://bbp.epfl.ch/ontologies/core/efeatures/SpikeDecayTime
:SpikeDecayTime rdf:type owl:Class ;
                rdfs:subClassOf <https://bbp.epfl.ch/ontologies/core/bmo/NeuronElectrophysiologicalFeature> ,
                                :NeuroElectroNeuronElectrophysiologicalFeature ;
                rdfs:label "Spike Decay Time"@en ;
                <http://www.w3.org/2004/02/skos/core#definition> "Time for spike to fall from peak to threshold, usually calculated as 10-90% decay time"@en ;
                <https://neuroshapes.org/units> "ms" .


###  https://bbp.epfl.ch/ontologies/core/efeatures/SpikeHalf-Width
:SpikeHalf-Width rdf:type owl:Class ;
                 rdfs:subClassOf <https://bbp.epfl.ch/ontologies/core/bmo/NeuronElectrophysiologicalFeature> ,
                                 :NeuroElectroNeuronElectrophysiologicalFeature ;
                 rdfs:label "Spike Half-Width"@en ;
                 <http://www.w3.org/2004/02/skos/core#definition> "Calculated as the AP duration at the membrane voltage halfway between AP threshold and AP peak. Most commonly calculated using first AP in train at rheobase. current."@en ;
                 <https://neuroshapes.org/units> "ms" .


###  https://bbp.epfl.ch/ontologies/core/efeatures/SpikeMaxDecaySlope
:SpikeMaxDecaySlope rdf:type owl:Class ;
                    rdfs:subClassOf <https://bbp.epfl.ch/ontologies/core/bmo/NeuronElectrophysiologicalFeature> ,
                                    :NeuroElectroNeuronElectrophysiologicalFeature ;
                    rdfs:label "Spike Max Decay Slope"@en ;
                    <http://www.w3.org/2004/02/skos/core#definition> "Maximum rate of rise of membrane voltage during spike falling phase"@en ;
                    <https://neuroshapes.org/units> "mV/ms" .


###  https://bbp.epfl.ch/ontologies/core/efeatures/SpikeMaxRiseSlope
:SpikeMaxRiseSlope rdf:type owl:Class ;
                   rdfs:subClassOf <https://bbp.epfl.ch/ontologies/core/bmo/NeuronElectrophysiologicalFeature> ,
                                   :NeuroElectroNeuronElectrophysiologicalFeature ;
                   rdfs:label "Spike Max Rise Slope"@en ;
                   <http://www.w3.org/2004/02/skos/core#definition> "Maximum rate of rise of membrane voltage during spike rising phase"@en ;
                   <https://neuroshapes.org/units> "mV/ms" .


###  https://bbp.epfl.ch/ontologies/core/efeatures/SpikePeak
:SpikePeak rdf:type owl:Class ;
           rdfs:subClassOf <https://bbp.epfl.ch/ontologies/core/bmo/NeuronElectrophysiologicalFeature> ,
                           :NeuroElectroNeuronElectrophysiologicalFeature ;
           rdfs:label "Spike Peak"@en ;
           <http://www.w3.org/2004/02/skos/core#definition> "Maximum voltage reached during AP"@en ;
           <https://neuroshapes.org/units> "mV" .


###  https://bbp.epfl.ch/ontologies/core/efeatures/SpikeRiseTime
:SpikeRiseTime rdf:type owl:Class ;
               rdfs:subClassOf <https://bbp.epfl.ch/ontologies/core/bmo/NeuronElectrophysiologicalFeature> ,
                               :NeuroElectroNeuronElectrophysiologicalFeature ;
               rdfs:label "Spike Rise Time"@en ;
               <http://www.w3.org/2004/02/skos/core#definition> "Time for spike to rise from threshold to peak, usually calculated as 10-90% rise time"@en ;
               <https://neuroshapes.org/units> "ms" .


###  https://bbp.epfl.ch/ontologies/core/efeatures/SpikeThreshold
:SpikeThreshold rdf:type owl:Class ;
                rdfs:subClassOf <https://bbp.epfl.ch/ontologies/core/bmo/NeuronElectrophysiologicalFeature> ,
                                :NeuroElectroNeuronElectrophysiologicalFeature ;
                rdfs:label "Spike Threshold"@en ;
                <http://www.w3.org/2004/02/skos/core#definition> "Voltage at which AP is initiated (as assessed by measuring rising slope of membrane voltage)"@en ;
                <https://neuroshapes.org/units> "mV" .


###  https://bbp.epfl.ch/ontologies/core/efeatures/SpikeWidth
:SpikeWidth rdf:type owl:Class ;
            rdfs:subClassOf <https://bbp.epfl.ch/ontologies/core/bmo/NeuronElectrophysiologicalFeature> ,
                            :NeuroElectroNeuronElectrophysiologicalFeature ;
            rdfs:label "Spike Width"@en ;
            <http://www.w3.org/2004/02/skos/core#definition> "Duration of AP, not explictly refered to as half-width"@en ;
            <https://neuroshapes.org/units> "ms" .


###  https://bbp.epfl.ch/ontologies/core/efeatures/SpontaneousFiringRate
:SpontaneousFiringRate rdf:type owl:Class ;
                       rdfs:subClassOf <https://bbp.epfl.ch/ontologies/core/bmo/NeuronElectrophysiologicalFeature> ,
                                       :NeuroElectroNeuronElectrophysiologicalFeature ;
                       rdfs:label "Spontaneous Firing Rate"@en ;
                       <http://www.w3.org/2004/02/skos/core#definition> "AP discharge rate in the absence of current injection or a stimulus"@en ;
                       <https://neuroshapes.org/units> "Hz" .


###  Generated by the OWL API (version 4.5.9.2019-02-01T07:24:44Z) https://github.com/owlcs/owlapi
